compiler/dsl/coq/ReflexQuark.v
@@ -1,0 +1,83 @@
+Require Import String.
+
+Require Import Reflex.
+Require Import ReflexBase.
+Require Import ReflexDenoted.
+Require Import ReflexVec.
+
+Open Scope string_scope.
+
+Definition NB_MSG : nat := 3.
+
+Definition PAYD : vvdesc NB_MSG := mk_vvdesc
+  [ ("Input",   [str_d])
+  ; ("Display", [str_d])
+  ; ("Quit",    [ ])
+  ].
+
+Definition KSTD : vdesc := mk_vdesc
+  [ fd_d (* curtab *)
+  ; fd_d (* screen *)
+  ].
+
+Definition IENVD : vdesc := mk_vdesc [].
+
+Inductive COMPT : Type := Tab | Screen | UserInput.
+
+Definition COMPS (t : COMPT) : comp :=
+  match t with
+  | Tab       => mk_comp "Tab"       "test/quark/tab.py"        []
+  | Screen    => mk_comp "Screen"    "test/quark/screen.py"     []
+  | UserInput => mk_comp "UserInput" "test/quark/user-input.py" []
+  end.
+
+Definition INIT : init_prog PAYD COMPT KSTD IENVD :=
+  [ fun s => Spawn _ _ _ _ Tab
+  ; fun s => Spawn _ _ _ _ Screen
+  ].
+
+Definition HANDLERS : handlers PAYD COMPT KSTD :=
+  (fun m =>
+    match tag PAYD m as _tm return
+      @sdenote _ SDenoted_vdesc (lkup_tag PAYD _tm) -> _
+    with
+
+(* Input *)
+    | None => fun pl =>
+       let envd := mk_vdesc [] in
+       existT (fun d => hdlr_prog PAYD COMPT KSTD d) envd (fun cfd s =>
+         let (input, _) := pl in
+         (fun st0 =>
+                                                 (* should be curtab *)
+            [ fun s => Send PAYD COMPT KSTD envd (CFd _) None (SLit _ input, tt)
+            ]
+         )
+       )
+
+(* Display *)
+    | Some None => fun pl =>
+       let envd := mk_vdesc [] in
+       existT (fun d => hdlr_prog PAYD COMPT KSTD d) envd (fun cfd s =>
+         let (url, _) := pl in
+         (fun st0 =>
+            [ fun s => Send PAYD COMPT KSTD envd (CFd _) (Some None) (SLit _ url, tt)
+            ]
+         )
+       )
+
+(* Quit *)
+    | Some (Some None) => fun pl =>
+       let envd := mk_vdesc [] in
+       existT (fun d => hdlr_prog PAYD COMPT KSTD d) envd (fun cfd s =>
+         let _ := pl in
+         (fun st0 =>
+           []
+         )
+       )
+
+    | Some (Some (Some bad)) => fun _ =>
+      match bad with end
+    end (pay PAYD m)
+  ).
+
+Definition main := mk_main (Build_spec NB_MSG PAYD IENVD KSTD COMPT COMPS INIT HANDLERS).
